Foundation/Modal/Neighborhood/Logic/END4.lean
@@ -1,6 +1,7 @@
 import Foundation.Modal.Neighborhood.Hilbert
 import Foundation.Modal.Neighborhood.Logic.END
 import Foundation.Modal.Neighborhood.Logic.E4
+import Foundation.Vorspiel.Set.Fin
 
 namespace LO.Modal
 
@@ -12,6 +13,13 @@ namespace Neighborhood
 
 protected class Frame.IsEND4 (F : Frame) extends F.IsEND, F.IsTransitive where
 protected abbrev FrameClass.END4 : FrameClass := { F | F.IsEND4 }
+
+instance : counterframe_2_3_5.IsEND where
+  contains_unit := by simp [Frame.box];
+  serial := by
+    rintro X x;
+    suffices X = {x}ᶜ ∨ X = Set.univ → ¬X = {x} ∧ ¬X = ∅ by simpa [Frame.box, Frame.dia];
+    rintro (rfl | rfl) <;> simp [Set.Fin2.ne_singleton_univ.symm];
 
 end Neighborhood
 
@@ -29,6 +37,8 @@ instance : Entailment.Consistent Modal.END4 := consistent_of_sound_frameclass Fr
 
 end END4
 
+
+
 instance : Modal.END ⪱ Modal.END4 := by
   constructor;
   . apply Hilbert.WithRE.weakerThan_of_subset_axioms;
@@ -37,6 +47,11 @@ instance : Modal.END ⪱ Modal.END4 := by
     use (Axioms.Four (.atom 0));
     constructor;
     . simp;
-    . sorry;
+    . apply Sound.not_provable_of_countermodel (𝓜 := FrameClass.END);
+      apply not_validOnFrameClass_of_exists_frame;
+      use counterframe_2_3_5;
+      constructor;
+      . apply Set.mem_setOf_eq.mpr; infer_instance;
+      . simp;
 
 end LO.Modal
